split lines

LeanCourse/Memory.lean
@@ -6,13 +6,15 @@ variable {ValTp IdTp ValSTp IdSTp : Type}
 
 inductive Memory (ValTp ValSTp IdSTp IdTp : Type) where
   | mtm
-  | write (mem : Memory ValTp ValSTp IdSTp IdTp) (id : IdT ValSTp IdSTp IdTp) (fld : FieldSelector ValSTp IdSTp) (val : ValT ValTp ValSTp IdSTp IdTp)
+  | write (mem : Memory ValTp ValSTp IdSTp IdTp) (id : IdT ValSTp IdSTp IdTp)
+    (fld : FieldSelector ValSTp IdSTp) (val : ValT ValTp ValSTp IdSTp IdTp)
   | add   (mem : Memory ValTp ValSTp IdSTp IdTp) (id : IdTp)
 
 namespace Memory
 
 @[simp] def read [DecidableEq ValSTp] [DecidableEq IdSTp] [DecidableEq IdTp]
-  [Inhabited ValTp] (mem : Memory ValTp ValSTp IdSTp IdTp) (id : IdT ValSTp IdSTp IdTp) (fld : FieldSelector ValSTp IdSTp) : ValT ValTp ValSTp IdSTp IdTp :=
+  [Inhabited ValTp] (mem : Memory ValTp ValSTp IdSTp IdTp) (id : IdT ValSTp IdSTp IdTp)
+  (fld : FieldSelector ValSTp IdSTp) : ValT ValTp ValSTp IdSTp IdTp :=
   match mem, id with
   | .mtm, _ => .val default
   | .write mem idM fldM val, _ => if idM = id && fldM = fld then val else read mem id fld
